\documentclass{article}
\usepackage[margin=0.75in]{geometry}
\usepackage{amsmath}
\usepackage{amssymb}
\usepackage{booktabs}
\usepackage{xintexpr}
\usepackage{multicol}

\setlength{\columnsep}{0.5cm}
\setlength{\columnseprule}{1pt}

\newcommand{\T}{1}
\newcommand{\F}{0}
\newcommand{\TF}[1]{\if1#1\T\else\F\fi}
\newcommand{\xintTF}[1]{\xintifboolexpr{#1}{\T}{\F}}

\newcommand{\logicrule}[2]{
\begin{array}{l}
#1 \\
\midrule
\therefore #2 \\
\end{array}
}

\newcommand{\problem}[2]{$\boxed{\text{#1 \##2}}$}
\newcommand{\subproblem}[1]{$\boxed{(#1)}$}
\newcommand{\RUS}{Rule of Universal Specification}
\newcommand{\RUG}{Rule of Universal Generalization}

\setlength\parindent{0pt}
\setlength\parskip{0em}

\begin{document}
\begin{multicols*}{2}

\problem{5}{1}

\subproblem{a} The problem lies in the first and second sentences. The
proof writer wanted to write the negation of the conclusion, but wrote
a different statement entirely. The problem statement is, in the
universe of the real numbers:

\[
\forall x\forall y((x+y=10)\rightarrow((x\ne 3)\wedge(y\ne 8)))
\]

The conclusion in particular is:

\[
(x\ne 3)\wedge(y\ne 8)
\]

If we negate that, we get:

\[
\neg((x\ne 3)\wedge(y\ne 8))
\] \[
\neg(x\ne 3)\vee\neg(y\ne 8)
\] \[
(x=3)\vee(y=8)
\]

We can see that the proof writer forgot to swap the $\wedge$ for a
$\vee$ when applying DeMorgan's Law.

\subproblem{b} Let $x=3$ and $y=7$. Therefore $x+y=10$, so the premise
is true. But the conclusion $(3\ne 3)\wedge(7\ne 8)$ is false, because
$3=3$.

\problem{5}{2}

Let the universe of discourse be the integers. We want to show that
$15|n$ iff $3|n$ and $5|n$. Written mathematically, we have:

\[
\forall n((15|n)\leftrightarrow((3|n)\wedge(5|n)))
\]

In order to prove this statement, we want to prove two statements:

\[\tag{a}
\forall n((15|n)\rightarrow((3|n)\wedge(5|n)))
\] \[\tag{b}
\forall n(((3|n)\wedge(5|n))\rightarrow(15|n))
\]

\subproblem{a} Let $n$ be an arbitrary integer. Assume $15|n$,
i.e. that $\exists{}a(n=15a)$. We can factor $15$ to get
$15=3\cdot{}5$. We can acknowledge the implication of this equivalence
with the expression $3|15$, or equivalently $\exists{}b(15=3b)$. By
substituting this expression for $15$ in the known value for $n$, we
get:

\[
n=(3b)a
\]

By using the associativity of the integers, we can rewrite this as:

\[
n=3(ba)
\]

If we let $c=ba$, which is an integer because the integers are closed
under multiplication, then we can rewrite this as $n=3c$. By the
definition of ``divides'', we can conclude that $3|n$.

We can apply the same steps as above, replacing $5$ for $3$, and
conclude that $5|n$. Because we have both $3|n$ and $5|n$, we have
$(3|n)\wedge(5|n)$, which is our conclusion. We have shown that this
statement is true for arbitrary $n$, and by the \RUG, we can conclude
that for any integer $n$, if $15|n$ then $3|n$ and $5|n$.

\subproblem{b} Let $n$ be an arbitrary integer. Assume $3|n$ and
$5|n$, or in other words, that $\exists{}b(n=3b)$ and
$\exists{}c(n=5c)$. We can set these two statements equal to each
other, to get:

\[
3b=5c
\]

If we solve for $b$, we get:

\[
b=\frac{5}{3}c
\]

Because we are working in the integers and we are working with an
integer $b$, the only way this expression can evaluate to an integer
is if $c$ is some multiple of $3$, or in other words, that $3|c$ and
$\exists{}x(c=3x)$. If we substitute this new value for $c$ into the
expression from $5|n$, we get:

\[
n=5(3x)
\]

We can redistribute the parenthesis because the multiplication follows
the rules of associativity in the integers, so we can rewrite it as:

\[
n=(5\cdot 3)x
\] \[
n=15x
\]

In other words, we have found that $n=15x$ for some integer $x$, which
is the definition for $15|n$. By the \RUG, we have shown that, since
this statement is true for arbitrary $n$, it must be true for any
integer $n$. We have concluded that for any integer $n$, if $3|n$ and
$5|n$, then $15|n$.

Finally, because we have proven statements (a) and (b), we have proven
the original statement.

\problem{5}{3}

Let the universe of discourse be the integers. We want to show whether
the following statement is true or not: if $m$ is even and $n$ is odd,
then $n^2-m^2=n+m$. One obvious counter example is any $n$ and $m$
chosen such that $n<m$, for example $(n,m)=(3,2)$. We can also show
that this is untrue for any chosen $n$ and $m$.

By the definitions of even and odd, we have that $\exists{}a(m=2a)$
and $\exists{}b(n=2b+1)$. If we expand the conclusion using these
values, we have that:

\[
(2a)^2+(2b+1)^2=(2a)-(2b+1)
\] \[
4a^2+4b^2+4b+1=2a-2b-1
\] \[
4a^2+4b^2+6b-2a+2=0
\] \[
2a^2+2b^2+3b-a+1=0
\] \[
2a^2-a+(2b^2+3b+1)=0
\]

Solving for $a$, we get:

\[
a=\dfrac{1\pm \sqrt{1^2-4\cdot 2\cdot (2b^2+3b+1)}}{2\cdot 2}
\] \[
a=\dfrac{1}{4}\pm\dfrac{\sqrt{1-16b^2-24b-4}}{4}
\]

Because we are working in the integers, the only way for this
expression to be true is if $4|a$ and consequently $\exists{}x(m=8x)$,
however this is not true in general. For example, if $m=2$, then
$\nexists{}x(2=8x)$.

\end{multicols*}
\end{document}
